New relation-based primitives, up to RFOR.

hol/primitivesScript.sml
@@ -116,4 +116,247 @@ val range_CONG = store_thm(
   >- (ONCE_REWRITE_TAC [FOR_def] >> srw_tac[ARITH_ss][]) >>
   rpt strip_tac >> srw_tac[ARITH_ss][FOR_nonzero]);
 
+(* relations *)
+val _ = type_abbrev ("mrel", ``:(num # num -> bool) # (num # num)``)
+val _ = overload_on("rsizex", ``\mr:mrel. FST (SND mr)``)
+val _ = overload_on("rsizey", ``\mr:mrel. SND (SND mr)``)
+
+val RIN_def = Define`
+  RIN xy mr ⇔ FST xy < rsizex mr ∧ SND xy < rsizey mr ∧ FST mr xy
+`;
+val _ = overload_on("IN", ``RIN``)
+
+val RIN_bounds = store_thm(
+  "RIN_bounds",
+  ``(x,y) ∈ mr ⇒ x < rsizex mr ∧ y < rsizey mr``,
+  simp[RIN_def]);
+
+val canonical_def = Define`
+  canonical mr ⇔
+    (case OLEAST mx. ∀x y. FST mr (x,y) ⇒ x < mx of
+         NONE => F
+       | SOME mx => rsizex mr = mx) ∧
+    (case OLEAST my. ∀x y. FST mr (x,y) ⇒ y < my of
+         NONE => F
+       | SOME my => rsizey mr = my)
+`;
+
+val mrEMPTY_def = Define`
+  mrEMPTY = (∅, (0,0))
+`;
+
+val IN_mrEMPTY = store_thm(
+  "IN_mrEMPTY",
+  ``p ∈ mrEMPTY ⇔ F``,
+  simp[mrEMPTY_def, RIN_def]);
+val _ = export_rewrites ["IN_mrEMPTY"]
+
+val rsize_mrEMPTY = store_thm(
+  "rsize_mrEMPTY",
+  ``rsizex mrEMPTY = 0 ∧ rsizey mrEMPTY = 0``,
+  simp[mrEMPTY_def]);
+val _ = export_rewrites ["rsize_mrEMPTY"]
+
+val mrEMPTY_canonical = store_thm(
+  "mrEMPTY_canonical",
+  ``canonical mrEMPTY``,
+  simp[canonical_def, mrEMPTY_def]);
+
+val _ = prove(
+  ``¬canonical (∅, 1, 0)``,
+  simp[canonical_def]);
+
+val complete_mr_def = Define`
+  complete_mr n = ((λ(x,y). x < n ∧ y < n), n, n)
+`;
+
+val rsize_complete_mr = store_thm(
+  "rsize_complete_mr",
+  ``rsizex (complete_mr n) = n ∧ rsizey (complete_mr n) = n``,
+  simp[complete_mr_def]);
+val _ = export_rewrites ["rsize_complete_mr"]
+
+val IN_complete_mr = store_thm(
+  "IN_complete_mr",
+  ``(x,y) ∈ complete_mr n ⇔ x < n ∧ y < n``,
+  simp[complete_mr_def, RIN_def]);
+val _ = export_rewrites ["IN_complete_mr"]
+
+val complete_mr_canonical = store_thm(
+  "complete_mr_canonical",
+  ``canonical (complete_mr n)``,
+  simp[canonical_def, complete_mr_def] >> conj_tac >>
+  DEEP_INTRO_TAC whileTheory.OLEAST_INTRO >> simp[] >>
+  (conj_tac >- metis_tac[]) >> rpt strip_tac >>
+  `¬(n < n') ∧ ¬(n' < n)` by metis_tac [DECIDE ``¬(x < x)``] >>
+  decide_tac)
+
+val mrel_EQ = store_thm(
+  "mrel_EQ",
+  ``mr1 = mr2 ⇔
+      rsizex mr1 = rsizex mr2 ∧
+      rsizey mr1 = rsizey mr2 ∧
+      FST mr1 = FST mr2``,
+  simp[pairTheory.PAIR_FST_SND_EQ, EQ_IMP_THM]);
+
+val canonical_zero_size = store_thm(
+  "canonical_zero_size",
+  ``canonical mr ⇒ (rsizex mr = 0 ⇔ rsizey mr = 0)``,
+  simp[canonical_def] >>
+  DEEP_INTRO_TAC whileTheory.OLEAST_INTRO >> simp[] >>
+  strip_tac >>
+  DEEP_INTRO_TAC whileTheory.OLEAST_INTRO >> simp[] >>
+  strip_tac >> eq_tac >> strip_tac >> fs[] >>
+  REV_FULL_SIMP_TAC (srw_ss()) []
+  >- (`~(rsizey mr - 1 < rsizey mr)` by simp[] >>
+      decide_tac) >>
+  `~(rsizex mr - 1 < rsizex mr)` by simp[] >>
+  decide_tac)
+val _ = export_rewrites ["canonical_zero_size"]
+
+val canonical_zero_size_EMPTY = store_thm(
+  "canonical_zero_size_EMPTY",
+  ``canonical mr ⇒ (rsizey mr = 0 ⇔ mr = mrEMPTY)``,
+  simp[EQ_IMP_THM] >> rpt strip_tac >>
+  `rsizex mr = 0` by metis_tac [canonical_zero_size] >>
+  Q.UNDISCH_THEN `canonical mr` mp_tac >>
+  simp[mrel_EQ] >>
+  simp[mrEMPTY_def, FUN_EQ_THM, canonical_def, pairTheory.FORALL_PROD] >>
+  DEEP_INTRO_TAC whileTheory.OLEAST_INTRO >> simp[]);
+val _ = export_rewrites ["canonical_zero_size_EMPTY"]
+
+val nonzero_canonical_has_members = store_thm(
+  "nonzero_canonical_has_members",
+  ``canonical mr ∧ rsizex mr ≠ 0 ⇒ ∃x y. (x,y) ∈ mr``,
+  simp[RIN_def] >> spose_not_then strip_assume_tac >>
+  `rsizey mr ≠ 0` by metis_tac[canonical_zero_size] >>
+  Q.UNDISCH_THEN `canonical mr` mp_tac >>
+  simp[canonical_def] >>
+  Cases_on `∀x y. ¬FST mr (x,y)` >> simp[] >> fs[] >>
+  Cases_on `x < rsizex mr`
+  >- (`¬(y < rsizey mr)` by metis_tac[] >>
+      DISJ2_TAC >>
+      DEEP_INTRO_TAC whileTheory.OLEAST_INTRO >> simp[]) >>
+  DISJ1_TAC >>
+  DEEP_INTRO_TAC whileTheory.OLEAST_INTRO >> simp[])
+
+(* would be nice to prove:
+val canonical_mrs_unique = store_thm(
+  "canonical_mrs_unique",
+  ``canonical mr1 ∧ canonical mr2 ∧ (∀p. p ∈ mr1 ⇔ p ∈ mr2) ⇒ mr1 = mr2``,
+  strip_tac >> simp_tac (srw_ss()) [mrel_EQ] >>
+  Cases_on `FST mr1 = FST mr2` >> simp[]
+  >- (fs[RIN_def] >>
+      Cases_on `rsizex mr1 = rsizex mr2` >> fs[] >>
+      spose_not_then assume_tac >>
+      Cases_on `rsizex mr2 = 0` >> fs[]
+      >- metis_tac [canonical_zero_size]
+      >- (`rsizey mr2 ≠ 0 ∧ rsizey mr1 ≠ 0` by metis_tac[canonical_zero_size] >>
+          `∃x1 y1 x2 y2. (x1,y1) ∈ mr1 ∧ (x2,y2) ∈ mr2`
+            by metis_tac[nonzero_canonical_has_members] >>
+      first_x_assum (qspec_then `(0,MIN (rsizey mr1) (rsizey mr2))` mp_tac) >>
+      srw_tac[ARITH_ss][EQ_IMP_THM]
+      >- (
+  CONJ
+  spose_not_then strip_assume_tac >>
+*)
+
+val FINITE_RELN_HAS_MAXCOORDS = store_thm(
+  "FINITE_RELN_HAS_MAXCOORDS",
+  ``∀r. FINITE r ⇒
+        (∃mx. ∀x y. (x,y) ∈ r ⇒ x < mx) ∧
+        ∃my. ∀x y. (x,y) ∈ r ⇒ y < my``,
+  Induct_on `FINITE r` >> simp[] >> rpt strip_tac >>
+  `∃x y. e = (x,y)` by (Cases_on `e` >> simp[])
+  >- (qexists_tac `MAX mx (x + 1)` >>
+      asm_simp_tac (srw_ss() ++ boolSimps.DNF_ss) []) >>
+  qexists_tac `MAX my (y + 1)` >>
+  asm_simp_tac (srw_ss() ++ boolSimps.DNF_ss) []);
+
+val canonical_mrs_exists = store_thm(
+  "canonical_mrs_exists",
+  ``FINITE r ⇒ ∃mr. canonical mr ∧ ∀p. p ∈ mr ⇔ p ∈ r``,
+  strip_tac >> imp_res_tac FINITE_RELN_HAS_MAXCOORDS >>
+  qexists_tac `(r,
+                (LEAST mx. ∀x y. (x,y) ∈ r ⇒ x < mx),
+                (LEAST my. ∀x y. (x,y) ∈ r ⇒ y < my))` >>
+  conj_tac
+  >- (simp[canonical_def] >> conj_tac >>
+      DEEP_INTRO_TAC whileTheory.OLEAST_INTRO >> simp[] >>
+      fs[SPECIFICATION] >> (conj_tac >- metis_tac[]) >>
+      rpt strip_tac >>
+      DEEP_INTRO_TAC whileTheory.LEAST_ELIM >> simp[] >>
+      (conj_tac >- metis_tac[]) >>
+      qx_gen_tac `m` >> strip_tac >>
+      metis_tac[arithmeticTheory.LESS_LESS_CASES]) >>
+  simp[pairTheory.FORALL_PROD] >> fs[RIN_def, SPECIFICATION] >>
+  map_every qx_gen_tac [`x`, `y`] >>
+  DEEP_INTRO_TAC whileTheory.LEAST_ELIM >> conj_tac >- metis_tac[] >>
+  qx_gen_tac `n` >> rpt strip_tac >> fs[] >>
+  DEEP_INTRO_TAC whileTheory.LEAST_ELIM >> conj_tac >- metis_tac[] >>
+  qx_gen_tac `m` >> rpt strip_tac >> fs[] >> metis_tac[]);
+
+val mrel_at_x_def = Define`
+  mrel_at_x (mr:mrel) x =
+    REVERSE (FOR (0,rsizey mr) (λy l. if (x,y) ∈ mr then y::l else l) [])
+`;
+
+val mrel_at_y_def = Define`
+  mrel_at_y (mr:mrel) y =
+    REVERSE (FOR (0,rsizex mr) (λx l. if (x,y) ∈ mr then x::l else l) [])
+`;
+
+
+val mrel_at_x_thm = store_thm(
+  "mrel_at_x_thm",
+  ``mrel_at_x mr x = FILTER (λy. (x,y) ∈ mr) (GENLIST I (rsizey mr))``,
+  simp[mrel_at_x_def] >>
+  DEEP_INTRO_TAC FOR_RULE >>
+  qexists_tac `
+    λi a. i ≤ rsizey mr ∧ a = REVERSE (FILTER (λy. (x,y) ∈ mr) (GENLIST I i))`>>
+  srw_tac[ARITH_ss][]
+  >- simp[GSYM arithmeticTheory.ADD1, listTheory.GENLIST,
+          listTheory.FILTER_APPEND_DISTRIB]
+  >- simp[GSYM arithmeticTheory.ADD1, listTheory.GENLIST,
+          listTheory.FILTER_APPEND_DISTRIB] >>
+  `j = rsizey mr` by decide_tac >> simp[]);
+
+val xmrels_present = store_thm(
+  "xmrels_present",
+  ``MEM y (mrel_at_x mr x) ⇔ (x,y) ∈ mr``,
+  simp[mrel_at_x_thm, listTheory.MEM_FILTER,
+       listTheory.MEM_GENLIST] >>
+  metis_tac[RIN_bounds]);
+
+val mrel_at_y_thm = store_thm(
+  "mrel_at_y_thm",
+  ``mrel_at_y mr y = FILTER (λx. (x,y) ∈ mr) (GENLIST I (rsizex mr))``,
+  simp[mrel_at_y_def] >>
+  DEEP_INTRO_TAC FOR_RULE >>
+  qexists_tac `
+    λi a. i ≤ rsizex mr ∧ a = REVERSE (FILTER (λx. (x,y) ∈ mr) (GENLIST I i))`>>
+  srw_tac[ARITH_ss][]
+  >- simp[GSYM arithmeticTheory.ADD1, listTheory.GENLIST,
+          listTheory.FILTER_APPEND_DISTRIB]
+  >- simp[GSYM arithmeticTheory.ADD1, listTheory.GENLIST,
+          listTheory.FILTER_APPEND_DISTRIB] >>
+  `j = rsizex mr` by decide_tac >> simp[]);
+
+val ymrels_present = store_thm(
+  "ymrels_present",
+  ``MEM x (mrel_at_y mr y) ⇔ (x,y) ∈ mr``,
+  simp[mrel_at_y_thm, listTheory.MEM_FILTER,
+       listTheory.MEM_GENLIST] >>
+  metis_tac[RIN_bounds]);
+
+val _ = Hol_datatype`direction = X | Y`
+val RFOR_def = Define`
+  RFOR X f mr A =
+    FOR (0, rsizex mr)
+        (λx acc. FOLDL (λy acc. f (x,y) acc) acc (mrel_at_x mr x)) ∧
+  RFOR Y f mr A =
+    FOR (0, rsizey mr)
+        (λy acc. FOLDL (λx acc. f (x,y) acc) acc (mrel_at_y mr y))
+`
+
 val _ = export_theory();
